Add main lemma for successive merkle trees.

src/dafny/smart/MerkleTrees.dfy
@@ -16,9 +16,10 @@ include "helpers/Helpers.dfy"
 include "trees/Trees.dfy"
 include "trees/CompleteTrees.dfy"
 include "paths/PathInCompleteTrees.dfy"
+include "synthattribute/Siblings.dfy"
 include "synthattribute/RightSiblings.dfy"
 include "seqofbits/SeqOfBits.dfy"
-
+include "helpers/SeqHelpers.dfy"
 
 module MerkleTrees {
 
@@ -26,29 +27,14 @@ module MerkleTrees {
     import opened Trees
     import opened CompleteTrees
     import opened PathInCompleteTrees
+    import opened Siblings
     import opened RSiblings
     import opened SeqOfBits
+    import opened SeqHelpers
 
-    /**
-     *  
-     *  @param  l       A list of elements.
-     *  @param  root    A tree.
-     *  @param  default The default vakue for right-padding the tree leaves.
-     *
-     *  We assume leavesIn return an indexed from left to right list of leaves.
-     *
-     *  @todo           We can use another function that returns the values instead
-     *                  of collectleaves (returns the seq of values directly) and then
-     *                  no need for `x.v`.
-     */
-    predicate treeLeftmostLeavesMatchList<T>(l: seq<T>, root: Tree<T>, default: T)
-        requires |l| <= |leavesIn(root)|
-    {
-        forall i:: 
-            (0 <= i < |l| ==> l[i] == leavesIn(root)[i].v)
-            && 
-            (|l| <= i < |leavesIn(root)|  ==> leavesIn(root)[i].v == default)
-    }
+    ///////////////////////////////////////////////////////////////////////////
+    //  Main predicates and functiona.
+    ///////////////////////////////////////////////////////////////////////////
 
     /**
      *  Whether the tree is a Merkle Tree.
@@ -56,70 +42,21 @@ module MerkleTrees {
      *  The tree must be:
      *      1.  complete
      *      2.  the first |l| leftmost leaves hold the values of `l`
-     *      3.  the values on the internal nodes correspond to the value of
+     *      3.  the leaves after |l| hold a default value `default`, 
+     *      4.  the values on the internal nodes correspond to the value of
      *          synthesied attribute `f`.
+     *
+     *  @param  root    A tree.
+     *  @param  l       A list, with the value sof the leftmost leaves.
+     *  @param  f       A binary function.
+     *  @param  default A default value for the rightmost leaves. 
      */
     predicate isMerkle<T>(root: Tree<T>, l: seq<T>, f : (T, T) -> T, default: T) 
-        requires |l| <= |leavesIn(root)| || |l| <= power2(height(root))
+        requires |l|  <= power2(height(root))
     {
         isCompleteTree(root)
-        && |leavesIn(root)| == power2(height(root))
         && isDecoratedWith(f, root)
         && treeLeftmostLeavesMatchList(l, root, default)
-    }
-
-    /**
-     *  Whether the tree is a Merkle Tree for a given list of elements.
-     *  
-     *  @param  root    A complete tree.
-     *  @param  l       A list of values.
-     *  @param  f       A binary operation.
-     *  @returns        True if and only if the tree is decorated with f
-     *                  and the leaves's values agree with `l`.
-     *
-     *  The tree must be:
-     *      1.  complete
-     *      2.  the values on the internal nodes correspond to the value of
-     *          synthesised attribute `f`.
-     *      3.  the leaves (in-order) hold the values of `l`
-     *
-     *  @todo   Change the name at some point as Merkle is used for hash attribute.
-     */
-    predicate isMerkle2<T>(root: Tree<T>, l: seq<T>, f : (T, T) -> T) 
-        requires |l| == |leavesIn(root)|
-    {
-        isCompleteTree(root)
-        && isDecoratedWith(f, root)                                     
-        && forall i :: 0 <= i < |l| ==> l[i] == leavesIn(root)[i].v                
-    }
-
-    /**
-     *  For tree of height >= 1, Merkle projects onto lc and rc for 
-     *  split list. 
-     *  @param  root    A complete tree.
-     *  @param  l       A list of values.
-     *  @param  f       A binary operation.
-     *  @param  h       The height of the tree.
-     *  @returns        True if and only if the tree is decorated with f
-     *                  and the leaves's values agree with `l`.
-     *
-     */
-    lemma {:induction h} treeIsMerkleImpliesChildrenAreMerkle<T>(r: Tree<T>, l: seq<T>, f : (T, T) -> T, h : nat)
-        requires |l| == |leavesIn(r)|
-        requires isMerkle2(r, l, f)
-        requires h == height(r) >= 1
-        ensures |l| == power2(height(r) )
-        ensures match r 
-            case Node(_, lc, rc) =>
-                |leavesIn(lc)| == power2(height(r))/2
-                && |l[.. power2(height(r))/2]| <=  |leavesIn(lc)|
-                && isMerkle2(lc, l[..  power2(height(r))/2], f)
-                && |leavesIn(rc)| == power2(height(r))/2
-                && |l[power2(height(r))/2..]| <=  |leavesIn(rc)|
-                && isMerkle2(rc, l[power2(height(r))/2..], f)
-    {
-        reveal_power2();
-        childrenInCompTreesHaveHalfNumberOfLeaves(r, h);
     }
 
    /** 
@@ -135,17 +72,37 @@ module MerkleTrees {
     *   @param  d   A default value for the leaves not in `l`.
     */
     function {:axiom} buildMerkle<T>(l: seq<T>, h : nat, f : (T, T) -> T, d : T) : Tree<T> 
-        requires h >= 0
         /** Tree has enough leaves to store `l`. */
         requires |l| <= power2(h)      
 
         ensures height(buildMerkle(l, h, f, d)) == h
-        ensures isCompleteTree(buildMerkle(l, h, f, d))
-        ensures |leavesIn(buildMerkle(l, h, f, d))| == power2(h)
-        ensures isDecoratedWith(f, buildMerkle(l, h, f, d))
-        ensures treeLeftmostLeavesMatchList(l, buildMerkle(l, h, f, d), d)
-        ensures hasLeavesIndexedFrom(buildMerkle(l, h, f, d), 0)
+        ensures |leavesIn(buildMerkle(l, h, f, d))| == power2(h)  
+        ensures isMerkle(buildMerkle(l, h, f, d), l, f, d)
 
+    /**
+     *  The |l| leftmost leaves of root are equal to l.
+     *  
+     *  @param  l           A list of elements.
+     *  @param  root        A tree.
+     *  @param  default     The default value for right-padding the tree leaves.
+     *
+     *  We assume leavesIn return an indexed (from left to right) list of leaves.
+     */
+    predicate treeLeftmostLeavesMatchList<T>(l: seq<T>, root: Tree<T>, default: T)
+        requires isCompleteTree(root)
+        requires |l| <= power2(height(root))
+    {
+        completeTreeNumberLemmas(root);
+        assert(|l| <= |leavesIn(root)|);
+        forall i:: 
+            (0 <= i < |l| ==> l[i] == leavesIn(root)[i].v)
+            && 
+            (|l| <= i < |leavesIn(root)|  ==> leavesIn(root)[i].v == default)
+    }
+
+    ///////////////////////////////////////////////////////////////////////////
+    //  Main properties.
+    ///////////////////////////////////////////////////////////////////////////
 
     /**
      *  The right siblings of the path to the last element of the list are
@@ -170,6 +127,238 @@ module MerkleTrees {
         var p := natToBitList(|l| - 1, height(r));
         bitToNatToBitsIsIdentity(|l| - 1, height(r));
         assert(bitListToNat(p) == |l| - 1);
+        completeTreeNumberLemmas(r);
+        assert(|l| <= |leavesIn(r)|);        
         rightSiblingsOfLastPathAreDefault(p, r, |l| - 1, f, 0, d);
     }
+
+    /**
+     *  Left siblings relation in two adjacent trees.
+     *  The values of left siblings in MKL(l) for the path to leaf right after last(l), are equal
+     *  to the values of the left siblings of the path to [a] in MKL(l + [a]).
+     *
+     *  @param  h   The height of the trees.
+     *  @param  l   The list of values.
+     *  @param  a   The element inserted in the tree.
+     *  @param  r   A merkle tree for l.
+     *  @param  r'  A merkle tree for l + [a].
+     *  @param  f   The synthesised attribute to compute.
+     *  @param  d   The default value for type T.
+     *  @param  p   The path to the the |l|-th leaf.
+     *  @param  p'  The path to the the (|l| + 1)-th leaf.
+     */
+
+    lemma {:induction l} nextPathSameSiblingsInNextList<T>(h : nat, l: seq<T>, a : T, r : Tree<T>, r' : Tree<T>, f : (T, T) -> T, d : T, p : seq<bit>, p' : seq<bit>) 
+        /** The list does not fill up the leaves of the tree.  */
+        requires 0 <= |l| < power2(h) - 1
+
+        /** Trees requirements. */ 
+        requires 1 <= h == height(r) == height(r') == h 
+        requires isCompleteTree(r) && isCompleteTree(r')
+        requires hasLeavesIndexedFrom(r, 0) && hasLeavesIndexedFrom(r', 0)
+        requires isMerkle(r, l, f, d) && isMerkle(r', l + [a], f, d);
+
+        /** Path `p` is to the (|l| -1)-th leaf indexed |l| - 1, p` to the |l|-th leaf i.e indexed |l|. */
+        requires |l| >= 1 ==> p  == natToBitList(|l| - 1, h);
+        requires p' == natToBitList(|l|, h);
+        
+        /** if |l| >= 1 then `p` has a zero. */
+        /** And hence we can compute nextpath(p), which is p'. */
+        ensures |l| >= 1 ==> exists i :: 0 <= i < |p| && p[i] == 0
+        ensures |l| >= 1 ==> p' == nextPath(p)
+
+        /**  */
+        ensures 
+            (|l| >= 1 && forall i :: 0 <= i < |p'|  ==>
+                siblingValueAt(p', r', i + 1) == siblingValueAt(nextPath(p), r, i + 1)
+            )
+            ||
+            (|l| == 0 ==>  forall i :: 0 <= i < |p'| ==> p'[i] == 0)
+
+    {
+        if |l| == 0 {
+            //  In this case, p' is a path to first leaf indexed 0 and  p' = [0,0,0 ...0]
+            //  So the premise  p'[i] == 1 is always false
+            calc == {
+                bitListToNat(p');
+                bitListToNat(natToBitList(|l|, h));
+                { bitToNatToBitsIsIdentity(|l|, h); }
+                |l|;
+                0;
+            }
+            valueIsZeroImpliesAllZeroes(p');
+            assert(forall i :: 0 <= i < |p'| ==> 
+                p'[i] == 0
+            );
+        } else {
+            bitToNatToBitsIsIdentity(|l| - 1, h);
+            assert(bitListToNat(p) == |l| - 1);
+            bitToNatToBitsIsIdentity(|l|, h);
+            assert(bitListToNat(p') == |l|);
+
+            //  Show that p has a zero.
+            pathToNoLasthasZero(p);
+        
+            //  Show that p' is actually nextPath(p)
+            succIsNextPath(p, p');
+
+            //  Siblings values in nextPath(p) in r and p' in r' are related.
+            //  Prove pre-conditions for applying lemma siblingsInEquivTrees
+            var k := |l|;
+            //  k < |leavesIn(r)| == |leavesIn(r')| 
+            completeTreeNumberLemmas(r);
+            completeTreeNumberLemmas(r');
+            assert(k < |leavesIn(r)| == |leavesIn(r')| );
+
+            //  takeLeavesIn(r, k) == takeLeavesIn(r', k)
+            //  dropLeavesIn(r, k + 1) == dropLeavesIn(r', k + 1)
+            equivTreesSameLeaves(h, l, a, r, r', f, d);
+            assert(takeLeavesIn(r, k) == takeLeavesIn(r', k));
+            assert(dropLeavesIn(r, k + 1) == dropLeavesIn(r', k + 1));
+
+            //  bitListToNat(p') == k 
+            calc == {
+                bitListToNat(p');
+                bitListToNat(natToBitList(|l|, h));
+                { bitToNatToBitsIsIdentity(|l|, h); }
+                |l|;
+            }
+
+            //  Apply lemma siblingsInEquivTrees
+            assert(bitListToNat(p') == k);
+
+            reveal_siblingValueAt();
+            siblingsInEquivTrees(p', r, r', k, f, 0);
+            assert(forall i :: 0 <= i < |p'| ==> siblingValueAt(p', r, i + 1) == siblingValueAt(p', r', i + 1));
+        }
+    }
+
+    ///////////////////////////////////////////////////////////////////////////
+    //  Helper lemmas and functions.
+    ///////////////////////////////////////////////////////////////////////////
+
+    /**
+     *  MKL(l) and MKL(l + [a]) have same leaves upto from 0 to |l| - 1 and
+     *  from |l| + 1 to 2^{height(tree)}.
+     *
+     *  @param  h   The height of the trees.
+     *  @param  l   The list of values.
+     *  @param  a   The element inserted in the tree.
+     *  @param  r   A merkle tree for l.
+     *  @param  r'  A merkle tree for l + [a].
+     *  @param  f   The synthesised attribute to compute.
+     *  @param  d   The default value for type T.
+     */
+
+    lemma equivTreesSameLeaves<T>(h : nat, l: seq<T>, a : T, r : Tree<T>, r' : Tree<T>, f : (T, T) -> T, d : T) 
+        /** The list does not fill up the leaves of the tree.  */
+        requires 0 <= |l| < power2(h) - 1
+
+        /** Trees requirements. */ 
+        requires 1 <= h == height(r) == height(r') == h 
+        requires isCompleteTree(r) && isCompleteTree(r')
+        requires hasLeavesIndexedFrom(r, 0) && hasLeavesIndexedFrom(r', 0)
+        requires isMerkle(r, l, f, d) && isMerkle(r', l + [a], f, d);
+    
+        ensures |l| + 1 < |leavesIn(r)| == |leavesIn(r')|
+        ensures  takeLeavesIn(r, |l|) == takeLeavesIn(r', |l|)
+        ensures dropLeavesIn(r, |l| + 1) == dropLeavesIn(r', |l| + 1)
+    {
+        completeTreeNumberLemmas(r);
+        completeTreeNumberLemmas(r');
+        
+        //  All leaves have same index
+        forall (i : nat | 0 <= i < power2(h) - 1) 
+            ensures leavesIn(r)[i].index == leavesIn(r')[i].index
+        {
+            calc == {
+                leavesIn(r)[i].index ;
+                i;
+                leavesIn(r)[i].index ;
+            }
+        }
+
+        //  All leaves except at |l|  have the same value.
+        forall (i : nat | 0 <= i <  power2(h) - 1) 
+            ensures i != |l| ==> leavesIn(r)[i].v == leavesIn(r')[i].v
+        {
+            if i < |l| {
+                calc == {
+                    leavesIn(r)[i].v;
+                    l[i];
+                    leavesIn(r')[i].v;
+                }
+            } else if i > |l| {
+                 calc == {
+                    leavesIn(r)[i].v;
+                    d;
+                    leavesIn(r')[i].v;
+                }
+            }
+            calc == {
+                leavesIn(r)[i].index ;
+                i;
+                leavesIn(r)[i].index ;
+            }
+        }
+        reveal_takeLeavesIn();
+        reveal_dropLeavesIn();
+        assert  takeLeavesIn(r, |l|) == takeLeavesIn(r', |l|);
+        assert  dropLeavesIn(r, |l| + 1) == dropLeavesIn(r', |l| + 1);
+    }
+
+    /**
+     *  Whether the tree is a Merkle Tree for a given list of elements.
+     *  
+     *  @param  root    A complete tree.
+     *  @param  l       A list of values.
+     *  @param  f       A binary operation.
+     *  @returns        True if and only if the tree is decorated with f
+     *                  and the leaves's values agree with `l`.
+     *
+     *  The tree must be:
+     *      1.  complete
+     *      2.  the values on the internal nodes correspond to the value of
+     *          synthesised attribute `f`.
+     *      3.  the leaves (in-order) hold the values of `l`
+     *
+     *  @todo   Change the name at some point as Merkle is used for hash attribute.
+     */
+    // predicate isMerkle2<T>(root: Tree<T>, l: seq<T>, f : (T, T) -> T) 
+    //     requires |l| == |leavesIn(root)|
+    // {
+    //     isCompleteTree(root)
+    //     && isDecoratedWith(f, root)                                     
+    //     && forall i :: 0 <= i < |l| ==> l[i] == leavesIn(root)[i].v                
+    // }
+
+    /**
+     *  For tree of height >= 1, Merkle projects onto lc and rc for 
+     *  split list. 
+     *
+     *  @param  root    A complete tree.
+     *  @param  l       A list of values.
+     *  @param  f       A binary operation.
+     *  @param  h       The height of the tree.
+     *  @returns        True if and only if the tree is decorated with f
+     *                  and the leaves's values agree with `l`.
+     */
+    // lemma {:induction h} treeIsMerkleImpliesChildrenAreMerkle<T>(r: Tree<T>, l: seq<T>, f : (T, T) -> T, h : nat, d : T)
+    //     requires |l| == |leavesIn(r)|
+    //     requires isMerkle(r, l, f, d : T)
+    //     requires h == height(r) >= 1
+    //     ensures |l| == power2(height(r) )
+    //     ensures match r 
+    //         case Node(_, lc, rc) =>
+    //             |leavesIn(lc)| == power2(height(r))/2
+    //             && |l[.. power2(height(r))/2]| <=  |leavesIn(lc)|
+    //             && isMerkle(lc, l[..  power2(height(r))/2], f)
+    //             && |leavesIn(rc)| == power2(height(r))/2
+    //             && |l[power2(height(r))/2..]| <=  |leavesIn(rc)|
+    //             && isMerkle(rc, l[power2(height(r))/2..], f)
+    // {
+    //     reveal_power2();
+    //     childrenInCompTreesHaveHalfNumberOfLeaves(r, h);
+    // }
+    
 }
